identified bug where certain transitions are explored but not added to LTS

examples/Proc.v
@@ -1,13 +1,14 @@
 Require Import MEBI.loader.
 
-Inductive action : Set := | ASend | ARecv .
+Inductive action : Set := | ASend | ARecv | BSend | BRecv.
 
 Inductive term : Set :=
 | trec : term
 | tend : term
 | tfix : term -> term
 | tact : action -> term -> term
-| tpar : term -> term -> term
+| tpar : term -> term -> term (* parallel *)
+| topt : term -> term -> term (* choice between options *)
 .
 
 Fixpoint tsubst (t1 : term) (t2 : term) :=
@@ -17,20 +18,31 @@ Fixpoint tsubst (t1 : term) (t2 : term) :=
   | tfix t => tfix t
   | tact a t => tact a (tsubst t1 t)
   | tpar tl tr => tpar (tsubst t1 tl) (tsubst t1 tr)
+  | topt tl tr => topt (tsubst t1 tl) (tsubst t1 tr)
   end.
 
 (* true: "comm", false: "silent" *)
 Inductive termLTS : term -> bool -> term -> Prop :=
-| do_send : forall tl tr, termLTS (tpar (tact ASend tl) (tact ARecv tr))
-                            true  (tpar tl tr)
+(* syncrhonous communication, i.e., send/recv in parallel *)
+| do_senda : forall tl tr, termLTS (tpar (tact ASend tl) (tact ARecv tr))
+                             true  (tpar tl tr)
 
-| do_parl : forall a tl tl' tr,
-    termLTS tl a tl' ->
-    termLTS (tpar tl tr) a (tpar tl' tr)
+| do_sendb : forall tl tr, termLTS (tpar (tact BSend tl) (tact BRecv tr))
+                             true  (tpar tl tr)
 
-| do_parr : forall a tl tr tr',
-    termLTS tr a tr' ->
-    termLTS (tpar tl tr) a (tpar tl tr')
+(* non-deterministic choice between tl and tr *)
+| do_optl : forall a tl tr tl', termLTS tl a tl' ->
+                                termLTS (topt tl tr) a tl'
+
+| do_optr : forall a tl tr tr', termLTS tr a tr' ->
+                                termLTS (topt tl tr) a tr'
+
+(* non-deterministic parallel step *)
+| do_parl : forall a tl tl' tr, termLTS tl a tl' ->
+                                termLTS (tpar tl tr) a (tpar tl' tr)
+
+| do_parr : forall a tl tr tr', termLTS tr a tr' ->
+                                termLTS (tpar tl tr) a (tpar tl tr')
 
 (* These below capture "structural congruence": using "silent" transitions *)
 | do_fix : forall t,
@@ -46,11 +58,70 @@ Inductive termLTS : term -> bool -> term -> Prop :=
     termLTS (tpar (tpar t1 t2) t3) false (tpar t1 (tpar t2 t3))
 .
 
-Example proc0 := tfix trec.
-(* MeBi Show LTS Bounded 150 Of proc0 Using termLTS. *)
+(*************************************)
+(** Basic: No recursion or branches **)
+(*************************************)
+
+Example proc0_send0 := tact ASend tend. (* empty lts *)
+MeBi Show LTS Bounded 150 Of proc0_send0 Using termLTS.
+
+Example proc0_send1 := tpar (tact ASend tend)
+                            (tact ARecv tend).
+MeBi Show LTS Bounded 150 Of proc0_send1 Using termLTS.
+(* MeBi Dump "proc0_send1" LTS Bounded 150 Of proc0_send1 Using termLTS. *)
+
+Example proc0_send2 := tpar (tact ASend (tact ASend tend))
+                            (tact ARecv (tact ARecv tend)).
+MeBi Show LTS Bounded 150 Of proc0_send2 Using termLTS.
+
+Example proc0_send3 := tpar (tact ASend (tact BSend tend))
+                            (tact ARecv (tact BRecv tend)).
+MeBi Show LTS Bounded 150 Of proc0_send3 Using termLTS.
+
+Example proc0_send4 := tpar (tact BSend (tact ASend tend))
+                            (tact BRecv (tact ARecv tend)).
+MeBi Show LTS Bounded 150 Of proc0_send4 Using termLTS.
+
+
+(*************************************)
+(** Simple Recursion, no Branching ***)
+(*************************************)
+
+Example proc1_rec1 := tfix trec.
+MeBi Show LTS Bounded 150 Of proc1_rec1 Using termLTS.
+
+Example proc1_rec2 := tpar (tfix (tact ASend trec))
+                           (tfix (tact ARecv trec)).
+MeBi Show LTS Bounded 150 Of proc1_rec2 Using termLTS.
+
+Example proc1_rec3 := tpar (tfix (tact ASend (tact BSend trec)))
+                           (tfix (tact ARecv (tact BRecv trec))).
+MeBi Show LTS Bounded 150 Of proc1_rec3 Using termLTS.
+
+Example proc1_rec4 := tpar (tact ASend (tfix (tact BSend trec)))
+                           (tact ARecv (tfix (tact BRecv trec))).
+MeBi Show LTS Bounded 150 Of proc1_rec4 Using termLTS.
+
+
+(*************************************)
+(** Branching, no Recursion **********)
+(*************************************)
+
+
+(*************************************)
+(** Simple Branching and Recursion ***)
+(*************************************)
+
+
+(*************************************)
+(** Nested Branching and Recursion ***)
+(*************************************)
+
+
+
 
 Example proc1 := tpar (tfix (tact ASend trec)) (tfix (tact ARecv trec)).
-(* MeBi Show LTS Bounded 150 Of proc1 Using termLTS. *)
+MeBi Show LTS Bounded 150 Of proc1 Using termLTS.
 (* MeBi Dump "proc1" LTS Bounded 1000 Of proc1 Using termLTS. *)
 
 Example proc2 := tpar proc1 proc1.
